src/program_proof/simplepb/pb_definitions.v
@@ -342,14 +342,14 @@ Defined.
 Definition is_pb_host_pre ρ : (u64 -d> simplepb_system_names -d> simplepb_server_names -d> iPropO Σ) :=
   (λ host γ γsrv,
   ∃ γrpc,
-  handler_spec γrpc host (U64 0) (ApplyAsBackup_spec γ γsrv) ∗
-  handler_spec γrpc host (U64 1) (SetState_spec γ γsrv) ∗
-  handler_spec γrpc host (U64 2) (GetState_spec γ γsrv) ∗
-  handler_spec γrpc host (U64 3) (BecomePrimary_spec_pre γ γsrv ρ) ∗
-  handler_spec γrpc host (U64 4) (Apply_spec γ) ∗
-  handler_spec γrpc host (U64 6) (ApplyRo_spec γ) ∗
-  handler_spec γrpc host (U64 7) (IncreaseCommit_spec γ γsrv) ∗
-  handlers_dom γrpc {[ (U64 0) ; (U64 1) ; (U64 2) ; (U64 3) ; (U64 4) ; (U64 6) ; (U64 7) ]})%I
+  is_urpc_spec_pred γrpc host (U64 0) (ApplyAsBackup_spec γ γsrv) ∗
+  is_urpc_spec_pred γrpc host (U64 1) (SetState_spec γ γsrv) ∗
+  is_urpc_spec_pred γrpc host (U64 2) (GetState_spec γ γsrv) ∗
+  is_urpc_spec_pred γrpc host (U64 3) (BecomePrimary_spec_pre γ γsrv ρ) ∗
+  is_urpc_spec_pred γrpc host (U64 4) (Apply_spec γ) ∗
+  is_urpc_spec_pred γrpc host (U64 6) (ApplyRo_spec γ) ∗
+  is_urpc_spec_pred γrpc host (U64 7) (IncreaseCommit_spec γ γsrv) ∗
+  is_urpc_dom γrpc {[ (U64 0) ; (U64 1) ; (U64 2) ; (U64 3) ; (U64 4) ; (U64 6) ; (U64 7) ]})%I
 .
 
 Instance is_pb_host_pre_contr : Contractive is_pb_host_pre.
